proofs/verilog_arithmetic_module_proof/Adder/RCA/rca_04_trs.v
@@ -1,0 +1,69 @@
+Require Import Coq.micromega.Lia.
+Require Import Coq.ZArith.BinInt.
+Require Import Coq.Lists.List. Import ListNotations.
+Require Import Pfv.Lib.Lib. Import SZNotations.
+Require Import Pfv.Lang.Lang.
+Require Import common.Common.
+
+Require Import Verification.VerilogArithmeticModule.Adder.RCA.common_gen.
+Require Import Verification.VerilogArithmeticModule.Adder.RCA.fa_gen.
+Require Import Verification.VerilogArithmeticModule.Adder.RCA.fa_trs.
+Require Import Verification.VerilogArithmeticModule.Adder.RCA.rca_04_gen.
+
+Import Rca_04.
+Import HMapNotations.
+Import SFMonadNotations.
+
+(* Use the instances from rca_04_gen *)
+#[local] Existing Instance vid_t_c_impl.
+#[local] Existing Instance vid_ops_impl.
+
+#[local] Existing Instance SZ_sz_ops.
+#[local] Existing Instance hmap_array_ops.
+
+Module Rca_04Trs.
+  Section AbsOps.
+    Context `{SZ_OPS: sz_ops} `{ARRAY_OPS: array_ops hmap}.
+  
+    Import ListNotations.
+    Import HMapNotations.
+  
+    Definition trs_structured_sigT: {trs: forall (inputs: Inputs) (flops: Flops), (Updates * Outputs) |
+      is_module_trs M.m fmapEmpty etrs Inputs Flops (to_unstructured_trs update_to_state output_to_state trs)
+    }.
+    Proof.
+      destruct SZ_OPS eqn: Hsz_ops, ARRAY_OPS eqn: Harray_ops.
+      match (type of Hsz_ops) with | SZ_OPS = ?a => set (SZ_OPS' := a) end.
+      match (type of Harray_ops) with | ARRAY_OPS = ?a => set (ARRAY_OPS' := a) end.
+      clear Hsz_ops SZ_OPS ARRAY_OPS Harray_ops.
+
+      unshelve epose (trs := _ : Inputs -> Flops -> Updates * Outputs).
+      { intros i f. destruct i, f. split; econstructor; eapply _. }
+      exists trs.
+      red. unfold to_unstructured_trs. intros ???? Htrs. unfold format.
+      destruct (from_state inputs) as [[]|], (from_state flops) as [[]|] in *;
+      vm_compute in Htrs; injection Htrs as <- <-.
+      2-4: eauto.
+      eexists. split; [split|].
+      - eapply trsM_iff_rep_is_chain with (n := 3%nat).
+        cbv.
+        reflexivity.
+      - cbv. reflexivity.
+      - cbv. reflexivity.
+      all: cbv; reflexivity.
+    Defined.
+  
+    Definition trs_structured := proj1_sig trs_structured_sigT.
+  
+    Definition mtrs: MTrsOf M.m fmapEmpty etrs Inputs Flops.
+    Proof.
+      eapply mk_MTrsOf with (mtrsof_mtrs := (Build_MTrs _ _ (to_unstructured_trs _ _ trs_structured))).
+      1-2: vm_compute; reflexivity. unfold mtrs_func.
+      eapply (proj2_sig trs_structured_sigT).
+    Defined.
+  
+    #[global] Opaque trs_structured.
+  
+  End AbsOps.
+End Rca_04Trs.
+
